Move some code into libraries

src/program_proof/wal/abstraction.v
@@ -1,15 +1,18 @@
 From RecordUpdate Require Import RecordSet.
-Import RecordSetNotations.
 
-From Goose.github_com.mit_pdos.goose_nfsd Require Import wal.
+From stdpp Require Import gmap.
+From iris.algebra Require Import ofe.
 
-From Perennial.program_proof Require Import proof_prelude disk_lib.
+From Perennial.Helpers Require Import Integers.
+From Perennial.program_proof Require Import disk_lib.
+From Perennial.goose_lang Require Import ffi.disk.
 
 Module update.
   Record t :=
     mk { addr: u64;
          b: Block; }.
   Global Instance _eta: Settable _ := settable! mk <addr; b>.
+  Global Instance _witness: Inhabited t := populate (mk inhabitant inhabitant).
 End update.
 
 Canonical Structure updateO := leibnizO update.t.
@@ -57,40 +60,3 @@ Definition wal_wf (s : log_state.t) :=
         empty transactions *)
       int.val pos1 ≤ int.val pos2) ∧
   s.(log_state.installed_lb) ≤ s.(log_state.durable_lb) ≤ length s.(log_state.txns).
-
-
-Section heap.
-Context `{!heapG Σ}.
-Definition update_val (up:u64*Slice.t): val :=
-  (#(fst up), (slice_val (snd up), #()))%V.
-
-Theorem update_val_t u : val_ty (update_val u) (struct.t Update.S).
-Proof.
-  repeat constructor.
-  destruct u; rewrite /blockT; val_ty.
-Qed.
-
-Definition updates_slice (bk_s: Slice.t) (bs: list update.t): iProp Σ :=
-  ∃ bks, is_slice bk_s (struct.t Update.S) 1 (update_val <$> bks) ∗
-   [∗ list] _ ↦ b_upd;upd ∈ bks;bs , let '(update.mk a b) := upd in
-                                     is_block (snd b_upd) b ∗
-                                     ⌜fst b_upd = a⌝.
-
-Lemma updates_slice_len bk_s bs :
-  updates_slice bk_s bs -∗ ⌜int.val bk_s.(Slice.sz) = length bs⌝.
-Proof.
-  iIntros "Hupds".
-  iDestruct "Hupds" as (bks) "[Hbs Hbks]".
-  iDestruct (is_slice_sz with "Hbs") as %Hbs_sz.
-  iDestruct (big_sepL2_length with "Hbks") as %Hbks_len.
-  rewrite fmap_length in Hbs_sz.
-  iPureIntro.
-  rewrite -Hbks_len.
-  rewrite Hbs_sz.
-  destruct bk_s; simpl.
-  word.
-Qed.
-
-End heap.
-
-Hint Resolve update_val_t : val_ty.
