src/Helpers/ListLen.v
@@ -1,0 +1,11 @@
+From Coq Require Import List.
+From stdpp Require Import list vector.
+From Perennial.Helpers Require Import Integers.
+
+Hint Rewrite app_length @drop_length @take_length @fmap_length
+     @replicate_length : len.
+Hint Rewrite @vec_to_list_length : len.
+Hint Rewrite @insert_length : len.
+Hint Rewrite u64_le_length : len.
+
+Ltac len := autorewrite with len; try word.
