src/goose_lang/lib/control/control.v
@@ -1,0 +1,24 @@
+From Perennial.goose_lang Require Import notation.
+From Perennial.goose_lang Require Import proofmode.
+From Perennial.goose_lang Require Import lang.
+
+Set Default Proof Using "Type".
+
+Section goose_lang.
+Context `{ffi_sem: ext_semantics} `{!ffi_interp ffi} `{!heapG Σ}.
+
+(** A proof principle for if e { do_stuff(); } where do_stuff() is optional and
+does something irrelevant to the proof using resources R. Allows to re-use the
+proof for both branches, carrying on with resources R. *)
+Theorem wp_If_optional stk E (R: iProp Σ) (b: bool) e :
+  (∀ (Φ': val → iProp Σ), R -∗ ▷ (R -∗ Φ' #()) -∗ WP e @ stk; E {{ Φ' }}) -∗
+  ∀ Φ, R -∗ ▷ (R -∗ Φ #()) -∗ WP If #b e #() @ stk; E {{ Φ }}.
+Proof.
+  iIntros "Hwp" (Φ) "HR HΦ".
+  wp_if_destruct.
+  - wp_apply ("Hwp" with "[$HR]").
+    iFrame.
+  - iApply ("HΦ" with "HR").
+Qed.
+
+End goose_lang.
