src/program_proof/wal/circ_proof.v
@@ -3,13 +3,14 @@ From Perennial.algebra Require Import deletable_heap.
 From Perennial.algebra Require Import fmcounter.
 
 From RecordUpdate Require Import RecordSet.
+
 From Goose.github_com.mit_pdos.goose_nfsd Require Import wal.
-From Perennial.program_proof Require Import proof_prelude.
-From Perennial.program_proof Require Import wal.abstraction.
-From Perennial.program_proof Require Import marshal_proof util_proof.
-From Perennial.program_proof Require Import disk_lib.
 
 From Perennial.Helpers Require Import Transitions.
+From Perennial.program_proof Require Import proof_prelude disk_lib.
+From Perennial.program_proof Require Import wal.lib.
+From Perennial.program_proof Require Import marshal_proof util_proof.
+
 Existing Instance r_mbind.
 
 Module circΣ.
@@ -1376,7 +1377,7 @@ Proof.
     iFrame.
     iSplitL.
     { iSplit.
-      { destruct Hwf; len. }
+      { iPureIntro; destruct Hwf; len. }
       iExactEq "HdiskEnd2".
       f_equal.
       destruct Hwf; len. }
