src/program_proof/wal/lib.v
@@ -1,0 +1,94 @@
+From Goose.github_com.mit_pdos.goose_nfsd Require Import wal.
+
+From Perennial.program_proof Require Export wal.abstraction.
+From Perennial.program_proof Require Import proof_prelude disk_lib.
+
+Section heap.
+Context `{!heapG Σ}.
+Definition update_val (up:u64*Slice.t): val :=
+  (#(fst up), (slice_val (snd up), #()))%V.
+
+Theorem update_val_t u : val_ty (update_val u) (struct.t Update.S).
+Proof.
+  repeat constructor.
+  destruct u; rewrite /blockT; val_ty.
+Qed.
+
+Definition updates_slice (bk_s: Slice.t) (bs: list update.t): iProp Σ :=
+  ∃ bks, is_slice bk_s (struct.t Update.S) 1 (update_val <$> bks) ∗
+   [∗ list] _ ↦ b_upd;upd ∈ bks;bs , let '(update.mk a b) := upd in
+                                     is_block (snd b_upd) b ∗
+                                     ⌜fst b_upd = a⌝.
+
+Lemma updates_slice_len bk_s bs :
+  updates_slice bk_s bs -∗ ⌜int.val bk_s.(Slice.sz) = length bs⌝.
+Proof.
+  iIntros "Hupds".
+  iDestruct "Hupds" as (bks) "[Hbs Hbks]".
+  iDestruct (is_slice_sz with "Hbs") as %Hbs_sz.
+  iDestruct (big_sepL2_length with "Hbks") as %Hbks_len.
+  rewrite fmap_length in Hbs_sz.
+  iPureIntro.
+  rewrite -Hbks_len.
+  rewrite Hbs_sz.
+  destruct bk_s; simpl.
+  word.
+Qed.
+
+Theorem wp_SliceGet_updates stk E bk_s bs (i: u64) (u: update.t) :
+  {{{ updates_slice bk_s bs ∗ ⌜bs !! int.nat i = Some u⌝ }}}
+    SliceGet (struct.t Update.S) (slice_val bk_s) #i @ stk; E
+  {{{ uv, RET (update_val uv);
+      ⌜uv.1 = u.(update.addr)⌝ ∗
+      is_block uv.2 u.(update.b) ∗
+      (is_block uv.2 u.(update.b) -∗ updates_slice bk_s bs)
+  }}}.
+Proof.
+  iIntros (Φ) "[Hupds %Hlookup] HΦ".
+  iDestruct "Hupds" as (bks) "[Hbk_s Hbks]".
+  iDestruct (big_sepL2_lookup_2_some _ _ _ _ _ Hlookup with "Hbks")
+    as %[b_upd Hlookup_bs].
+  iDestruct (is_slice_small_acc with "Hbk_s") as "[Hbk_s Hbk_s_rest]".
+  wp_apply (wp_SliceGet with "[$Hbk_s]").
+  { iPureIntro.
+    rewrite list_lookup_fmap.
+    rewrite Hlookup_bs //. }
+  iIntros "[Hbk_s _]".
+  iDestruct ("Hbk_s_rest" with "Hbk_s") as "Hbk_s".
+  iApply "HΦ".
+  iDestruct (big_sepL2_lookup_acc with "Hbks") as "[Hbi Hbks]"; eauto.
+  destruct u as [a b]; simpl.
+  iDestruct "Hbi" as "[Hbi <-]".
+  iSplit; first by auto.
+  iFrame.
+  iIntros "Hbi".
+  iSpecialize ("Hbks" with "[$Hbi //]").
+  rewrite /updates_slice.
+  iExists _; iFrame.
+Qed.
+
+Theorem wp_copyUpdateBlock stk E (u: u64 * Slice.t) b :
+  {{{ is_block (snd u) b }}}
+    copyUpdateBlock (update_val u) @ stk; E
+  {{{ (s':Slice.t), RET (slice_val s'); is_block (snd u) b ∗ is_block s' b }}}.
+Proof.
+  iIntros (Φ) "Hb HΦ".
+  destruct u as [a s]; simpl.
+  wp_call.
+  wp_apply wp_new_slice; first by auto.
+  iIntros (s') "Hs'".
+  iDestruct (is_slice_to_small with "Hs'") as "Hs'".
+  wp_pures.
+  wp_apply (wp_SliceCopy_full with "[$Hb $Hs']").
+  { iPureIntro.
+    autorewrite with len.
+    rewrite length_Block_to_vals.
+    reflexivity. }
+  iIntros "(Hs&Hs')".
+  wp_pures.
+  iApply ("HΦ" with "[$]").
+Qed.
+
+End heap.
+
+Hint Resolve update_val_t : val_ty.
